cfrontend/Cshmgenproof.v
@@ -15,7 +15,7 @@
 Require Import Coqlib Errors Maps Integers Floats.
 Require Import AST Linking.
 Require Import Values Events Memory Globalenvs Smallstep.
-Require Import Ctypes Cop Clight Cminor Csharpminor.
+Require Import Ctypes Ctyping Cop Clight Cminor Csharpminor.
 Require Import Cshmgen.
 
 (** * Relational specification of the transformation *)
@@ -996,6 +996,26 @@ Proof.
   eapply make_memcpy_correct with (b := b) (v := Vptr b' ofs'); eauto.
 Qed.
 
+Lemma make_normalization_correct:
+  forall e le m a v t,
+  eval_expr ge e le m a v ->
+  wt_val v t ->
+  eval_expr ge e le m (make_normalization t a) v.
+Proof.
+  intros. destruct t; simpl; auto. inv H0.
+- destruct i; simpl in H3.
+  + destruct s; econstructor; eauto; simpl; congruence.
+  + destruct s; econstructor; eauto; simpl; congruence.
+  + auto.
+  + econstructor; eauto; simpl; congruence.
+- auto.
+- destruct i.
+  + destruct s; econstructor; eauto. 
+  + destruct s; econstructor; eauto.
+  + auto.
+  + econstructor; eauto.
+Qed.
+
 End CONSTRUCTORS.
 
 (** * Basic preservation invariants *)
@@ -1360,7 +1380,16 @@ Inductive match_cont: composite_env -> type -> nat -> nat -> Clight.cont -> Csha
       match_cont cu.(prog_comp_env) (Clight.fn_return f) nbrk' ncnt' k tk ->
       match_cont ce tyret nbrk ncnt
                  (Clight.Kcall id f e le k)
-                 (Kcall id tf te le tk).
+                 (Kcall id tf te le tk)
+  | match_Kcall_normalize: forall ce tyret nbrk ncnt nbrk' ncnt' f e k id a tf te le tk cu,
+      linkorder cu prog ->
+      transl_function cu.(prog_comp_env) f = OK tf ->
+      match_env e te ->
+      match_cont cu.(prog_comp_env) (Clight.fn_return f) nbrk' ncnt' k tk ->
+      (forall v e le m, wt_val v tyret -> le!id = Some v -> eval_expr tge e le m a v) ->
+      match_cont ce tyret nbrk ncnt
+                 (Clight.Kcall (Some id) f e le k)
+                 (Kcall (Some id) tf te le (Kseq (Sset id a) tk)).
 
 Inductive match_states: Clight.state -> Csharpminor.state -> Prop :=
   | match_state:
@@ -1377,14 +1406,15 @@ Inductive match_states: Clight.state -> Csharpminor.state -> Prop :=
       forall fd args k m tfd tk targs tres cconv cu ce
           (LINK: linkorder cu prog)
           (TR: match_fundef cu fd tfd)
-          (MK: match_cont ce Tvoid 0%nat 0%nat k tk)
+          (MK: match_cont ce tres 0%nat 0%nat k tk)
           (ISCC: Clight.is_call_cont k)
           (TY: type_of_fundef fd = Tfunction targs tres cconv),
       match_states (Clight.Callstate fd args k m)
                    (Callstate tfd args tk m)
   | match_returnstate:
-      forall res k m tk ce
-          (MK: match_cont ce Tvoid 0%nat 0%nat k tk),
+      forall res tres k m tk ce
+          (MK: match_cont ce tres 0%nat 0%nat k tk)
+          (WT: wt_val res tres),
       match_states (Clight.Returnstate res k m)
                    (Returnstate res tk m).
 
@@ -1442,7 +1472,9 @@ Proof.
 - (* set *)
   auto.
 - (* call *)
-  simpl in TR. destruct (classify_fun (typeof e)); monadInv TR. auto.
+  simpl in TR. destruct (classify_fun (typeof e)); monadInv TR.
+  unfold make_funcall.
+  destruct o; auto; destruct Conventions1.return_value_needs_normalization; auto.
 - (* builtin *)
   auto.
 - (* seq *)
@@ -1500,24 +1532,26 @@ End FIND_LABEL.
 (** Properties of call continuations *)
 
 Lemma match_cont_call_cont:
-  forall ce' tyret' nbrk' ncnt' ce tyret nbrk ncnt k tk,
+  forall ce' nbrk' ncnt' ce tyret nbrk ncnt k tk,
   match_cont ce tyret nbrk ncnt k tk ->
-  match_cont ce' tyret' nbrk' ncnt' (Clight.call_cont k) (call_cont tk).
+  match_cont ce' tyret nbrk' ncnt' (Clight.call_cont k) (call_cont tk).
 Proof.
   induction 1; simpl; auto.
-  constructor.
-  econstructor; eauto.
+- apply match_Kstop.
+- eapply match_Kcall; eauto.
+- eapply match_Kcall_normalize; eauto.
 Qed.
 
 Lemma match_cont_is_call_cont:
-  forall ce tyret nbrk ncnt k tk ce' tyret' nbrk' ncnt',
+  forall ce tyret nbrk ncnt k tk ce' nbrk' ncnt',
   match_cont ce tyret nbrk ncnt k tk ->
   Clight.is_call_cont k ->
-  match_cont ce' tyret' nbrk' ncnt' k tk /\ is_call_cont tk.
+  match_cont ce' tyret nbrk' ncnt' k tk /\ is_call_cont tk.
 Proof.
   intros. inv H; simpl in H0; try contradiction; simpl.
-  split; auto; constructor.
-  split; auto; econstructor; eauto.
+  split; auto; apply match_Kstop.
+  split; auto; eapply match_Kcall; eauto.
+  split; auto; eapply match_Kcall_normalize; eauto.
 Qed.
 
 (** The simulation proof *)
@@ -1549,19 +1583,44 @@ Proof.
 
 - (* call *)
   revert TR. simpl. case_eq (classify_fun (typeof a)); try congruence.
-  intros targs tres cc CF TR. monadInv TR. inv MTR.
+  intros targs tres cc CF TR. monadInv TR.
   exploit functions_translated; eauto. intros (cu' & tfd & FIND & TFD & LINK').
   rewrite H in CF. simpl in CF. inv CF.
-  econstructor; split.
-  apply plus_one. econstructor; eauto.
-  eapply transl_expr_correct with (cunit := cu); eauto.
-  eapply transl_arglist_correct with (cunit := cu); eauto.
-  erewrite typlist_of_arglist_eq by eauto.
-  eapply transl_fundef_sig1; eauto.
-  rewrite H3. auto.
-  econstructor; eauto.
-  eapply match_Kcall with (ce := prog_comp_env cu') (cu := cu); eauto.
-  simpl. auto.
+  set (sg := {| sig_args := typlist_of_arglist al targs;
+                sig_res := rettype_of_type tres;
+                sig_cc := cc |}) in *.
+  assert (SIG: funsig tfd = sg).
+  { unfold sg; erewrite typlist_of_arglist_eq by eauto.
+    eapply transl_fundef_sig1; eauto. rewrite H3; auto. }
+  assert (EITHER: tk' = tk /\ ts' = Scall optid sg x x0
+               \/ exists id, optid = Some id /\
+                  tk' = tk /\ ts' = Sseq (Scall optid sg x x0)
+                                         (Sset id (make_normalization tres (Evar id)))).
+  { unfold make_funcall in MTR.
+    destruct optid. destruct Conventions1.return_value_needs_normalization.
+    inv MTR. right; exists i; auto.
+    inv MTR; auto.
+    inv MTR; auto. }
+  destruct EITHER as [(EK & ES) | (id & EI & EK & ES)]; rewrite EK, ES.
+  + (* without normalization of return value *)
+    econstructor; split.
+    apply plus_one. eapply step_call; eauto.
+    eapply transl_expr_correct with (cunit := cu); eauto.
+    eapply transl_arglist_correct with (cunit := cu); eauto.
+    econstructor; eauto.
+    eapply match_Kcall with (ce := prog_comp_env cu') (cu := cu); eauto.
+    exact I.
+  + (* with normalization of return value *)
+    subst optid.
+    econstructor; split.
+    eapply plus_two. apply step_seq. eapply step_call; eauto. 
+    eapply transl_expr_correct with (cunit := cu); eauto.
+    eapply transl_arglist_correct with (cunit := cu); eauto.
+    traceEq.
+    econstructor; eauto.
+    eapply match_Kcall_normalize  with (ce := prog_comp_env cu') (cu := cu); eauto.
+    intros. eapply make_normalization_correct; eauto. constructor; eauto.
+    exact I.
 
 - (* builtin *)
   monadInv TR. inv MTR.
@@ -1658,6 +1717,7 @@ Proof.
   eapply match_env_free_blocks; eauto.
   eapply match_returnstate with (ce := prog_comp_env cu); eauto.
   eapply match_cont_call_cont. eauto.
+  constructor.
 
 - (* return some *)
   monadInv TR. inv MTR.
@@ -1667,6 +1727,7 @@ Proof.
   eapply match_env_free_blocks; eauto.
   eapply match_returnstate with (ce := prog_comp_env cu); eauto.
   eapply match_cont_call_cont. eauto.
+  apply wt_val_casted. eapply cast_val_is_casted; eauto.
 
 - (* skip call *)
   monadInv TR. inv MTR.
@@ -1675,6 +1736,7 @@ Proof.
   apply plus_one. apply step_skip_call. auto.
   eapply match_env_free_blocks; eauto.
   eapply match_returnstate with (ce := prog_comp_env cu); eauto.
+  constructor.
 
 - (* switch *)
   monadInv TR.
@@ -1738,20 +1800,33 @@ Proof.
   simpl. econstructor; eauto.
   unfold transl_function. rewrite EQ; simpl. rewrite EQ1; simpl. auto.
   constructor.
+  replace (fn_return f) with tres. eassumption.
+  simpl in TY. unfold type_of_function in TY. congruence. 
 
 - (* external function *)
   inv TR.
   exploit match_cont_is_call_cont; eauto. intros [A B].
   econstructor; split.
-  apply plus_one. constructor. eauto.
+  apply plus_one. constructor.
   eapply external_call_symbols_preserved; eauto. apply senv_preserved.
   eapply match_returnstate with (ce := ce); eauto.
+  apply has_rettype_wt_val. 
+  replace (rettype_of_type tres0) with (sig_res (ef_sig ef)).
+  eapply external_call_well_typed_gen; eauto.
+  rewrite H5. simpl. simpl in TY. congruence.
 
 - (* returnstate *)
   inv MK.
-  econstructor; split.
-  apply plus_one. constructor.
-  econstructor; eauto. simpl; reflexivity. constructor.
+  + (* without normalization *)
+    econstructor; split.
+    apply plus_one. constructor.
+    econstructor; eauto. simpl; reflexivity. constructor.
+  + (* with normalization *)
+    econstructor; split.
+    eapply plus_three. econstructor. econstructor. constructor.
+    simpl. apply H13. eauto. apply PTree.gss.
+    traceEq.
+    simpl. rewrite PTree.set2. econstructor; eauto. simpl; reflexivity. constructor.
 Qed.
 
 Lemma transl_initial_states:
